add_comm proof (admitted)

ems/ModSem.v
@@ -22,8 +22,6 @@ Section MODSEM.
   Record t: Type := mk {
     state : Type;
     init_st : state;
-    (* init_st : Any.t; *)
-    (* fnsems : gname -> option (Any.t -> itree Es Any.t); *)
     fnsems : gname -> option (Any.t -> itree (Es state) Any.t)
   }
   .
@@ -60,7 +58,11 @@ Section INTERP.
 
   Context `{CONF: EMSConfig}.
 
-  Definition initial_itr: itree eventE Any.t :=
+  Definition initial_itr (P: option Prop): itree eventE Any.t :=
+    match P with
+    | None => Ret tt
+    | Some P' => assume (<<WF: P'>>)
+    end;;; 
     snd <$> interp_Es prog (prog (Call "main" initial_arg)) (init_st ms).
 
   Let state: Type := itree eventE Any.t.
@@ -231,16 +233,35 @@ Section INTERP.
   Next Obligation. inv STEP; ss. Qed.
   Next Obligation. inv STEP; ss. Qed.
 
-  Definition compile :=
-    compile_itree (initial_itr).
-  End INTERP.
+  Definition compile P: semantics:=
+    compile_itree (initial_itr P).
 
+  Lemma initial_itr_not_wf P
+        (WF: ~ P)
+        tr
+    :
+      Beh.of_program (compile_itree (initial_itr (Some P))) tr.
+  Proof.
+    eapply Beh.ub_top. pfold. econsr; ss; et. rr. ii; ss.
+    unfold initial_itr, assume in *. rewrite bind_bind in STEP.
+    eapply step_trigger_take_iff in STEP. des. subst. ss.
+  Qed.
 
-End MODSEM.
+  Lemma compile_not_wf P
+        (WF: ~ P)
+        tr
+    :
+      Beh.of_program (compile (Some P)) tr.
+  Proof.
+    eapply initial_itr_not_wf; et.
+  Qed.
+
+End INTERP.
+
 
 
 Section ADD.
-  Variable M1 M2 : ModSem.t.
+  Variable M1 M2 : t.
 
   Definition emb_l : forall X, Es (state M1) X -> Es (state M1 * state M2) X  :=
     lmap fstl.
@@ -251,30 +272,13 @@ Section ADD.
   Definition add_fnsems : gname -> option (Any.t -> itree _ Any.t) :=
     fun fn =>
       match M1.(fnsems) fn, M2.(fnsems) fn with
-      | Some fn_body, None => Some (fun args => map_event emb_l (fn_body args))
-      | None, Some fn_body => Some (fun args => map_event emb_r (fn_body args))
-      (* Some _, Some _ => UB *)
+      | Some fn_body, None => Some (fun args => translate emb_l (fn_body args))
+      | None, Some fn_body => Some (fun args => translate emb_r (fn_body args))
+      | Some _, Some _ => Some (fun args => triggerUB)
       | _, _ => None
       end.
 
-  (* Definition add_fnsems (ms1 ms2: t) : gname -> option (Any.t -> itree _ Any.t) :=
-    fun fn =>
-      match (fnsems ms1) fn, (fnsems ms2) fn with
-      | Some fn_body, None => Some (fun args => map_event emb_l (fn_body args))
-      | None, Some fn_body => Some (fun args => map_event emb_r (fn_body args))
-      (* Some _, Some _ => UB *)
-      | _, _ => None
-      end.   *)
-
-  (* Definition add (ms1 ms2 : t) : t :=
-    {|
-      init_st := Any.pair (init_st ms1) (init_st ms2);
-      fnsems := add_fnsems ms1 ms2;
-
-    |}. *)
-
-
-  Definition add : ModSem.t :=
+  Definition add : t :=
   {|
     state := state M1 * state M2;
     init_st := (init_st M1, init_st M2);
@@ -283,15 +287,55 @@ Section ADD.
 
 End ADD.
 
+Lemma itr_snd
+        (S0 S1 A: Type)
+        (st0: S0) (st1: S1) (a: A)
+        (itr0: itree eventE (S0 * A)) (itr1: itree eventE (S1 * A)) 
+        (I0: itr0 = Ret (st0, a))
+        (I1: itr1 = Ret (st1, a))
+:
+  snd <$> itr0 = snd <$> itr1
+.
+Proof. 
+  simpl. rewrite I0, I1. unfold ITree.map. rewrite bind_ret_l. rewrite bind_ret_l. et.
+Qed.
+(* 
+Lemma add_fnsems_comm
+      ms0 ms1 fn
+:
+      (add_fnsems ms0 ms1 fn) = (add_fnsems ms1 ms0 fn)
+. *)
+
+
+Lemma interp_Es_vis
+T R st p (st0: st)
+(* (e: Es Σ) *)
+(c: callE T) (k: T -> itree (Es st) R)
+:
+interp_Es p (Vis (c|)%sum k) st0 = tau;; (interp_Es p (ITree.bind (p _ c) k) st0) 
+.
+Proof. 
+unfold interp_Es, interp_sE.
+rewrite interp_mrec_bind. grind.
+Admitted. 
+(* f_equal. 
+
+Check interp_mrec_trigger.
+change (` x : T <- ITree.trigger (c|)%sum;; k x) with (ITree.bind (ITree.trigger ((c|)%sum)) k).
+grind. Qed. *)
+
+
+
 Context {CONF: EMSConfig}.
 
 Let add_comm_aux
     ms0 ms1 stl0 str0
+    P
     (SIM: stl0 = str0)
   :
-    <<COMM: Beh.of_state (compile (add ms0 ms1)) stl0
+    <<COMM: Beh.of_state (compile (add ms0 ms1) P) stl0
             <1=
-            Beh.of_state (compile (add ms1 ms0)) str0>>
+            Beh.of_state (compile (add ms1 ms0) P) str0>>
 .
 Proof.
   subst. revert str0. pcofix CIH. i. pfold.
@@ -324,41 +368,98 @@ Proof.
   r. eapply prop_ext. split; i; auto.
 Qed. *)
 
+
+
 Theorem add_comm
         ms0 ms1
-        (* (P0 P1: Prop) (IMPL: P1 -> P0) *)
+        (P0 P1: Prop) (IMPL: P1 -> P0)
         (* (WF: wf (add ms1 ms0)) *)
   :
-    <<COMM: Beh.of_program (compile (add ms0 ms1)) <1= Beh.of_program (compile (add ms1 ms0))>>
+    <<COMM: Beh.of_program (compile (add ms0 ms1) (Some P0)) <1= Beh.of_program (compile (add ms1 ms0) (Some P1))>>
 .
 Proof.
-  ii. r. eapply add_comm_aux; et. rp; et. ss. f_equal. cbn. unfold initial_itr. f_equal.
-  Admitted.
-(*   
   destruct (classic (P1)); cycle 1.
-  { ii. eapply initial_itr_not_wf; et. }
+  { ii. eapply initial_itr_not_wf;et. }
   replace P0 with P1.
   2: { eapply prop_ext. split; auto. }
-  ii. ss. r in PR. r. eapply add_comm_aux; et.
+  ii. ss. r in PR. r. eapply add_comm_aux. et.
   rp; et. clear PR. ss. cbn. unfold initial_itr. f_equal.
-  { extensionality u. destruct u. f_equal.
-    replace (@interp_Es Any.t (prog (add ms1 ms0))) with (@interp_Es Any.t (prog (add ms0 ms1))).
-    { f_equal.
-      { ss. f_equal. f_equal. eapply alist_permutation_find.
-        { inv WF. et. }
-        { eapply Permutation_app_comm. }
-      }
-      { unfold initial_p_state. extensionality mn. ss.
-        erewrite alist_permutation_find; et.
-        { inv WF. ss. }
-        { eapply Permutation_app_comm. }
-      }
+  
+  extensionality u. destruct u.
+  apply bisimulation_is_eq. generalize "main" as fn.
+  ginit. gcofix CIH.
+  simpl. unfold ITree.map. repeat (rewrite interp_Es_bind; rewrite bind_bind).  
+  unfold unwrapU. unfold add_fnsems. i.
+  destruct (fnsems ms0 fn); cycle 1.
+  {
+    destruct (fnsems ms1 fn); cycle 1.
+    - rewrite ! interp_Es_bind. rewrite ! interp_Es_triggerUB.
+      gstep. unfold triggerUB. grind. 
+      rewrite ! bind_trigger; s.
+      econs. i. destruct v.  
+    - rewrite ! interp_Es_bind. rewrite ! interp_Es_ret. rewrite ! bind_ret_l.
+      rewrite ! interp_Es_bind. grind.
+      generalize (i initial_arg).
+      gcofix CIH'. i.
+      rewrite (itree_eta_ i0). 
+      destruct (observe i0).
+      + rewrite (bisimulation_is_eq _ _ (translate_ret (emb_l ms1 ms0) r0)).
+        rewrite (bisimulation_is_eq _ _ (translate_ret (emb_r ms0 ms1) r0)).
+        rewrite ! interp_Es_ret. rewrite ! bind_ret_l.
+        rewrite ! interp_Es_ret. rewrite ! bind_ret_l.
+        gstep. econs. et.
+
+      + 
+        rewrite (bisimulation_is_eq _ _ (translate_tau (emb_l ms1 ms0) t0)).
+        rewrite (bisimulation_is_eq _ _ (translate_tau (emb_r ms0 ms1) t0)).
+        rewrite ! interp_Es_tau. rewrite ! bind_tau.
+        gstep. econs. gfinal. left. apply CIH'.
+      + rewrite (bisimulation_is_eq _ _ (translate_vis (emb_l ms1 ms0) _ e k)).
+        rewrite (bisimulation_is_eq _ _ (translate_vis (emb_r ms0 ms1) _ e k)).
+        destruct e.
+        * unfold emb_l, emb_r, lmap. clear CIH'.
+          rewrite ! interp_Es_vis. destruct c.
+          gstep. grind. econs. gupaco.
+          apply eqit_clo_bind; et. Print eqit_bind_clo.
+          econs.
+          { admit. }
+          { admit. }
+        * admit.
+
+       
+          (* right. 
+          apply CIH.
+
+          eassert (Y := (interp_Es_callE _ _ c)).
+          unfold trigger in Y.
+          rewrite interp_Es_bind in Y.
+          unfold subevent in Y. unfold resum, ReSum_inl, ">>>" in Y. 
+          unfold emb_l, lmap. unfold Cat_IFun, inl_, Inl_sum1, resum, ReSum_id, id_, Id_IFun in Y.
+          rewrite Y.
+          Print Subevent.vis. Check subevent.
+          rewrite Y.
+        rewrite (interp_Es_callE _ _ c) (emb_l ms1 ms0 (c|)%sum)). *)
+
     }
-    f_equal. unfold prog. extensionality T. extensionality e. destruct e.
-    f_equal. f_equal. symmetry. eapply alist_permutation_find; et.
-    { inv WF. ss. }
-    { eapply Permutation_app_comm. } 
-  }
+    {
+      admit.
+    }
+Admitted.
+
+  (* revert ms0 ms1. pcofix CIH. i.
+  pfold.
+
+  
+
+
+
+
+
+  simpl. unfold ITree.map. repeat (rewrite interp_Es_bind; rewrite bind_bind).
+  unfold unwrapU. unfold add_fnsems.
+  
+  
+  
 Qed. *)
 
 Lemma add_assoc' ms0 ms1 ms2:
@@ -379,25 +480,26 @@ Proof. Admitted.
 Qed. *)
 
 Theorem add_assoc
-        ms0 ms1 ms2
+        ms0 ms1 ms2 P
   :
-    <<COMM: Beh.of_program (compile (add ms0 (add ms1 ms2))) <1=
-            Beh.of_program (compile (add (add ms0 ms1) ms2))>>
+    <<COMM: Beh.of_program (compile (add ms0 (add ms1 ms2)) P) <1=
+            Beh.of_program (compile (add (add ms0 ms1) ms2) P)>>
 .
 Proof. 
   rewrite add_assoc_eq. ss.
 Qed.
 
 Theorem add_assoc_rev
-        ms0 ms1 ms2
+        ms0 ms1 ms2 P
   :
-    <<COMM: Beh.of_program (compile (add ms0 (add ms1 ms2))) <1=
-            Beh.of_program (compile (add (add ms0 ms1) ms2))>>
+    <<COMM: Beh.of_program (compile (add ms0 (add ms1 ms2)) P) <1=
+            Beh.of_program (compile (add (add ms0 ms1) ms2) P)>>
 .
 Proof.
   rewrite add_assoc_eq. ss.
 Qed.
 
+End MODSEM.
 End ModSem.
 
 
@@ -431,7 +533,7 @@ Context {CONF: EMSConfig}.
 
 
 Definition compile (md: t): semantics :=
-  ModSem.compile_itree (ModSem.initial_itr md.(enclose)).
+  ModSem.compile_itree (ModSem.initial_itr md.(enclose) (Some (wf md))).
 
 
 (*** wf about modsem is enforced in the semantics ***)
@@ -540,6 +642,9 @@ Qed. *)
 Definition add_list (xs: list t): t :=
   fold_right add empty xs
 .
+
+(* Lemma add_list_single: forall (x: t), add_list [x] = x.
+Proof. ii; cbn. rewrite add_empty_r. refl. Qed. *)
 
 Definition add_list_cons
           x xs
@@ -964,11 +1069,11 @@ Arguments Sk.add: simpl never.
 Arguments Sk.wf: simpl never.
 Coercion Sk.load_skenv: Sk.t >-> SkEnv.t.
 Global Opaque Sk.load_skenv.
-Variable st: Type.
+(* Variable st: Type. *)
 
 (*** TODO: Move to ModSem.v ***)
 Lemma interp_Es_unwrapU
-      prog R (st0: st) (r: option R)
+      S prog R (st0: S) (r: option R)
   :
     interp_Es prog (unwrapU r) st0 = r <- unwrapU r;; Ret (st0, r)
 .
@@ -979,7 +1084,7 @@ Proof.
 Qed.
 
 Lemma interp_Es_unwrapN
-      prog R (st0: st) (r: option R)
+      S prog R (st0: S) (r: option R)
   :
     interp_Es prog (unwrapN r) st0 = r <- unwrapN r;; Ret (st0, r)
 .
@@ -990,7 +1095,7 @@ Proof.
 Qed.
 
 Lemma interp_Es_assume
-      prog (st0: st) (P: Prop)
+      S prog (st0: S) (P: Prop)
   :
     interp_Es prog (assume P) st0 = assume P;;; tau;; tau;; Ret (st0, tt)
 .
@@ -1004,7 +1109,7 @@ Proof.
 Qed.
 
 Lemma interp_Es_guarantee
-      prog (st0: st) (P: Prop)
+      S prog (st0: S) (P: Prop)
   :
     interp_Es prog (guarantee P) st0 = guarantee P;;; tau;; tau;; Ret (st0, tt)
 .
@@ -1024,7 +1129,7 @@ Qed.
 Require Import Red IRed.
 Section AUX.
   Lemma interp_Es_ext
-        prog R (itr0 itr1: itree _ R) (st0: st)
+        S prog R (itr0 itr1: itree _ R) (st0: S)
     :
       itr0 = itr1 -> interp_Es prog itr0 st0 = interp_Es prog itr1 st0
   .
