ems/SimModSem.v
@@ -54,13 +54,13 @@ Section SIM.
       fn varg k_src k_tgt
       (WF: wf w0 (st_src0, st_tgt0))
       (K: forall w1 vret st_src1 st_tgt1 (WLE: le w0 w1) (WF: wf w1 (st_src1, st_tgt1)),
-          sim_itree _ _ _ _ wf RR true true w (st_src1, k_src vret) (st_tgt1, k_tgt vret))
+          sim_itree _ _ _ _ wf RR false false w (st_src1, k_src vret) (st_tgt1, k_tgt vret))
     :
       _sim_itree sim_itree wf RR i_src0 i_tgt0 w (st_src0, trigger (Call fn varg) >>= k_src)
                  (st_tgt0, trigger (Call fn varg) >>= k_tgt)
 
   | sim_itree_syscall
-      i_src0 i_tgt0 w0 (st_src0: st_src) (st_tgt0: st_tgt)
+      i_src0 i_tgt0 w0 st_src0 st_tgt0
       fn varg rvs k_src k_tgt
       (K: forall vret,
           sim_itree _ _ _ _ wf RR true true w0 (st_src0, k_src vret) (st_tgt0, k_tgt vret))
@@ -116,17 +116,17 @@ Section SIM.
 
   | sim_itree_supdate_src
       i_src0 i_tgt0 w0 (st_src0: st_src) (st_tgt0: st_tgt)
-      k_src i_tgt
-      (run: st_src -> st_src * _ )
-      (K: _sim_itree sim_itree wf RR true i_tgt0 w0 (fst (run st_src0), k_src tt) (st_tgt0, i_tgt))
+      X k_src i_tgt
+      (run: st_src -> st_src * X )
+      (K: _sim_itree sim_itree wf RR true i_tgt0 w0 (fst (run st_src0), k_src (snd (run st_src0))) (st_tgt0, i_tgt))
     :
-      _sim_itree sim_itree wf RR i_src0 i_tgt0 w0 (st_src0, trigger (SUpdate run) >>= k_src)(st_tgt0, i_tgt)  
+      _sim_itree sim_itree wf RR i_src0 i_tgt0 w0 (st_src0, trigger (SUpdate run) >>= k_src) (st_tgt0, i_tgt)  
 
   | sim_itree_supdate_tgt
       i_src0 i_tgt0 w0 (st_src0: st_src) (st_tgt0: st_tgt)
-      i_src k_tgt
-      (run: st_tgt -> st_tgt * _ )
-      (K: _sim_itree sim_itree wf RR i_src0 true w0 (st_src0, i_src) (fst (run st_tgt0), k_tgt tt))
+      X i_src k_tgt
+      (run: st_tgt -> st_tgt * X )
+      (K: _sim_itree sim_itree wf RR i_src0 true w0 (st_src0, i_src) (fst (run st_tgt0), k_tgt (snd (run st_tgt0))))
     :
       _sim_itree sim_itree wf RR i_src0 i_tgt0 w0 (st_src0, i_src) (st_tgt0, trigger (SUpdate run) >>= k_tgt)
 
@@ -158,7 +158,7 @@ Section SIM.
             fn varg k_src k_tgt
             (WF: wf w0 (st_src0, st_tgt0))
             (K: forall w1 vret st_src1 st_tgt1 (WLE: le w0 w1) (WF: wf w1 (st_src1, st_tgt1)),
-                sim_itree _ _ _ _ wf RR true true w (st_src1, k_src vret) (st_tgt1, k_tgt vret)),
+                sim_itree _ _ _ _ wf RR false false w (st_src1, k_src vret) (st_tgt1, k_tgt vret)),
             P i_src0 i_tgt0 w (st_src0, trigger (Call fn varg) >>= k_src)
               (st_tgt0, trigger (Call fn varg) >>= k_tgt))
         (SYSCALL: forall
@@ -206,17 +206,17 @@ Section SIM.
               (st_tgt0, trigger (Take X) >>= k_tgt))
         (SUPDATESRC: forall
             i_src0 i_tgt0 w0 (st_src0: st_src) (st_tgt0: st_tgt)
-            k_src i_tgt
-            (run: st_src -> st_src * _ )
-            (K: _sim_itree sim_itree wf RR true i_tgt0 w0 (fst (run st_src0), k_src tt) (st_tgt0, i_tgt))
-            (IH: P true i_tgt0 w0 (fst (run st_src0), k_src tt) (st_tgt0, i_tgt)),
+            X k_src i_tgt
+            (run: st_src -> st_src * X )
+            (K: _sim_itree sim_itree wf RR true i_tgt0 w0 (fst (run st_src0), k_src (snd (run st_src0))) (st_tgt0, i_tgt))
+            (IH: P true i_tgt0 w0 (fst (run st_src0), k_src (snd (run st_src0))) (st_tgt0, i_tgt)),
             P i_src0 i_tgt0 w0 (st_src0, trigger (SUpdate run) >>= k_src) (st_tgt0, i_tgt))
         (SUPDATETGT: forall
             i_src0 i_tgt0 w0 (st_src0: st_src) (st_tgt0: st_tgt)
-            i_src k_tgt
-            (run: st_tgt -> st_tgt * _ )
-            (K: _sim_itree sim_itree wf RR i_src0 true w0 (st_src0, i_src) (fst (run st_tgt0), k_tgt tt))
-            (IH: P i_src0 true w0 (st_src0, i_src) (fst (run st_tgt0), k_tgt tt)),
+            X i_src k_tgt
+            (run: st_tgt -> st_tgt * X )
+            (K: _sim_itree sim_itree wf RR i_src0 true w0 (st_src0, i_src) (fst (run st_tgt0), k_tgt (snd (run st_tgt0))))
+            (IH: P i_src0 true w0 (st_src0, i_src) (fst (run st_tgt0), k_tgt (snd (run st_tgt0)))),
             P i_src0 i_tgt0 w0 (st_src0, i_src) (st_tgt0, trigger (SUpdate run) >>= k_tgt))
         (PROGRESS: forall
             i_src0 i_tgt0 w0 (st_src0: st_src) (st_tgt0: st_tgt) i_src i_tgt
@@ -245,7 +245,7 @@ Section SIM.
 
   Qed.
 
-  Definition sim_itree {st_src st_tgt} o_src o_tgt w0 (wf: world -> (st_src * st_tgt) -> Prop) :=
+  Definition sim_itree {st_src st_tgt} o_src o_tgt w0 (wf: world -> (st_src * st_tgt) -> Prop): _ -> _ -> Prop :=
     paco11 _sim_itree bot11 _ _ _ _ wf (lift_rel w0 wf (@eq Any.t)) o_src o_tgt w0.
 
   Lemma sim_itree_mon: monotone11 _sim_itree.
@@ -258,10 +258,10 @@ Section SIM.
   Hint Constructors _sim_itree.
   Hint Unfold sim_itree.
   Hint Resolve sim_itree_mon: paco.
-  Hint Resolve cpn8_wcompat: paco.
+  Hint Resolve cpn11_wcompat: paco.
 
   Lemma sim_itree_ind
-        {st_src st_tgt} R_src R_tgt (RR: st_src -> st_tgt -> R_src -> R_tgt -> Prop) (wf: world -> (st_src * st_tgt) -> Prop)
+        {st_src st_tgt} R_src R_tgt (wf: world -> (st_src * st_tgt) -> Prop) (RR: st_src -> st_tgt -> R_src -> R_tgt -> Prop) 
         (P: bool -> bool -> world -> st_src * itree (Es st_src) R_src -> st_tgt * itree (Es st_tgt) R_tgt -> Prop)
         (RET: forall
             i_src0 i_tgt0 w0 st_src0 st_tgt0
@@ -273,7 +273,7 @@ Section SIM.
             fn varg k_src k_tgt
             (WF: wf w0 (st_src0, st_tgt0))
             (K: forall w1 vret st_src1 st_tgt1 (WLE: le w0 w1) (WF: wf w1 (st_src1, st_tgt1)),
-                paco11 _sim_itree bot11 _ _ _ _ wf RR true true w (st_src1, k_src vret) (st_tgt1, k_tgt vret)),
+                paco11 _sim_itree bot11 _ _ _ _ wf RR false false w (st_src1, k_src vret) (st_tgt1, k_tgt vret)),
             P i_src0 i_tgt0 w (st_src0, trigger (Call fn varg) >>= k_src)
               (st_tgt0, trigger (Call fn varg) >>= k_tgt))
         (SYSCALL: forall
@@ -321,17 +321,18 @@ Section SIM.
               (st_tgt0, trigger (Take X) >>= k_tgt))
         (SUPDATESRC: forall
             i_src0 i_tgt0 w0 (st_src0: st_src) (st_tgt0: st_tgt)
-            k_src i_tgt
-            (run: st_src -> st_src * _ )
-            (K: paco11 _sim_itree bot11 _ _ _ _ wf RR true i_tgt0 w0 (fst (run st_src0), k_src tt) (st_tgt0, i_tgt))
-            (IH: P true i_tgt0 w0 (fst (run st_src0), k_src tt) (st_tgt0, i_tgt)),
+            X k_src i_tgt
+            (run: st_src -> st_src * X )
+            (K: paco11 _sim_itree bot11 _ _ _ _ wf RR true i_tgt0 w0 (fst (run st_src0), k_src (snd (run st_src0))) (st_tgt0, i_tgt))
+            (IH: P true i_tgt0 w0 (fst (run st_src0), k_src (snd (run st_src0))) (st_tgt0, i_tgt)),
             P i_src0 i_tgt0 w0 (st_src0, trigger (SUpdate run) >>= k_src) (st_tgt0, i_tgt))
         (SUPDATETGT: forall
             i_src0 i_tgt0 w0 (st_src0: st_src) (st_tgt0: st_tgt)
-            i_src k_tgt
-            (run: st_tgt -> st_tgt * _ )
-            (K: paco11 _sim_itree bot11 _ _ _ _ wf RR i_src0 true w0 (st_src0, i_src) (fst (run st_tgt0), k_tgt tt))
-            (IH: P i_src0 true w0 (st_src0, i_src) (fst (run st_tgt0), k_tgt tt)),
+            X i_src k_tgt
+            (run: st_tgt -> st_tgt * X )
+            (K: paco11 _sim_itree bot11 _ _ _ _ wf RR i_src0 true w0 (st_src0, i_src) (fst (run st_tgt0), k_tgt (snd (run st_tgt0))))
+            (IH:  P i_src0 true w0 (st_src0, i_src) (fst (run st_tgt0), k_tgt (snd (run st_tgt0)))),
+
             P i_src0 i_tgt0 w0 (st_src0, i_src) (st_tgt0, trigger (SUpdate run) >>= k_tgt))       
         (PROGRESS: forall
             i_src0 i_tgt0 w0 (st_src0: st_src) (st_tgt0: st_tgt)
@@ -377,7 +378,7 @@ Section SIM.
       fn varg k_src k_tgt
       (WF: wf w0 (st_src0, st_tgt0))
       (K: forall w1 vret st_src1 st_tgt1 (WLE: le w0 w1) (WF: wf w1 (st_src1, st_tgt1)),
-          sim_itree _ _ _ _ wf RR true true w (st_src1, k_src vret) (st_tgt1, k_tgt vret))
+          sim_itree _ _ _ _ wf RR false false w (st_src1, k_src vret) (st_tgt1, k_tgt vret))
     :
       sim_itree_indC sim_itree wf RR i_src0 i_tgt0 w (st_src0, trigger (Call fn varg) >>= k_src)
                      (st_tgt0, trigger (Call fn varg) >>= k_tgt)
@@ -436,17 +437,17 @@ Section SIM.
   
   | sim_itree_indC_supdate_src
       i_src0 i_tgt0 w0 (st_src0: st_src) (st_tgt0: st_tgt)
-      k_src i_tgt
-      (run: st_src -> st_src * _ )
-      (K: sim_itree _ _ _ _ wf RR true i_tgt0 w0 (fst (run st_src0), k_src tt) (st_tgt0, i_tgt))
+      X k_src i_tgt
+      (run: st_src -> st_src * X )
+      (K: sim_itree _ _ _ _ wf RR true i_tgt0 w0 (fst (run st_src0), k_src (snd (run st_src0))) (st_tgt0, i_tgt))
     :
       sim_itree_indC sim_itree wf RR i_src0 i_tgt0 w0 (st_src0, trigger (SUpdate run) >>= k_src) (st_tgt0, i_tgt)
 
   | sim_itree_indC_supdate_tgt
       i_src0 i_tgt0 w0 (st_src0: st_src) (st_tgt0: st_tgt)
-      i_src k_tgt
-      (run: st_tgt -> st_tgt * _ )
-      (K: sim_itree _ _ _ _ wf RR i_src0 true w0 (st_src0, i_src) (fst (run st_tgt0), k_tgt tt))
+      X i_src k_tgt
+      (run: st_tgt -> st_tgt * X )
+      (K: sim_itree _ _ _ _ wf RR i_src0 true w0 (st_src0, i_src) (fst (run st_tgt0), k_tgt (snd (run st_tgt0))))
     :
       sim_itree_indC sim_itree wf RR i_src0 i_tgt0 w0 (st_src0, i_src) (st_tgt0, trigger (SUpdate run) >>= k_tgt)
   .
@@ -472,8 +473,8 @@ Section SIM.
     { econs 7; eauto. i. eapply sim_itree_mon; eauto. i. eapply rclo11_base. eauto. }
     { econs 8; eauto. i. eapply sim_itree_mon; eauto. i. eapply rclo11_base. eauto. }
     { econs 9; eauto. des. esplits; eauto. eapply sim_itree_mon; eauto. i. eapply rclo11_base. eauto. }
-    { econs 10; eauto. eapply sim_itree_mon; eauto. i. eapply rclo11_base. eauto.  }
-    { econs 11; eauto. eapply sim_itree_mon; eauto. i. eapply rclo11_base. eauto.  }
+    { econs 10; eauto. des. esplits; eauto. eapply sim_itree_mon; eauto. i. eapply rclo11_base. eauto.  }
+    { econs 11; eauto. des. esplits; eauto.  eapply sim_itree_mon; eauto. i. eapply rclo11_base. eauto.  }
   Qed.
 
   Variant sim_itreeC (r g: forall (st_src st_tgt R_src R_tgt: Type) (wf: world -> (st_src * st_tgt) -> Prop) (RR: st_src -> st_tgt -> R_src -> R_tgt -> Prop), bool -> bool -> world -> st_src * itree (Es st_src) R_src -> st_tgt * itree (Es st_tgt) R_tgt -> Prop)
@@ -490,7 +491,7 @@ Section SIM.
       fn varg k_src k_tgt
       (WF: wf w0 (st_src0, st_tgt0))
       (K: forall w1 vret st_src1 st_tgt1 (WLE: le w0 w1) (WF: wf w1 (st_src1, st_tgt1)),
-          g _ _ _ _ wf RR true true w (st_src1, k_src vret) (st_tgt1, k_tgt vret))
+          g _ _ _ _ wf RR false false w (st_src1, k_src vret) (st_tgt1, k_tgt vret))
     :
       sim_itreeC r g wf RR i_src0 i_tgt0 w (st_src0, trigger (Call fn varg) >>= k_src)
                  (st_tgt0, trigger (Call fn varg) >>= k_tgt)
@@ -548,17 +549,17 @@ Section SIM.
                  (st_tgt0, trigger (Take X) >>= k_tgt)
   | sim_itreeC_supdate_src
       i_src0 i_tgt0 w0 (st_src0: st_src) (st_tgt0: st_tgt)
-      k_src i_tgt
-      (run: st_src -> st_src * _ )
-      (K: r _ _ _ _ wf RR true i_tgt0 w0 (fst (run st_src0), k_src tt) (st_tgt0, i_tgt))
+      X k_src i_tgt
+      (run: st_src -> st_src * X )
+      (K: r _ _ _ _ wf RR true i_tgt0 w0 (fst (run st_src0), k_src (snd (run st_src0))) (st_tgt0, i_tgt))
     :
       sim_itreeC r g wf RR i_src0 i_tgt0 w0 (st_src0, trigger (SUpdate run) >>= k_src) (st_tgt0, i_tgt)
 
   | sim_itreeC_supdate_tgt
       i_src0 i_tgt0 w0 (st_src0: st_src) (st_tgt0: st_tgt)
-      i_src k_tgt
-      (run: st_tgt -> st_tgt * _)
-      (K: r _ _ _ _ wf RR i_src0 true w0 (st_src0, i_src) (fst (run st_tgt0), k_tgt tt))
+      X i_src k_tgt
+      (run: st_tgt -> st_tgt * X )
+      (K: r _ _ _ _ wf RR i_src0 true w0 (st_src0, i_src) (fst (run st_tgt0), k_tgt (snd (run st_tgt0))))
     :
       sim_itreeC r g wf RR i_src0 i_tgt0 w0 (st_src0, i_src) (st_tgt0, trigger (SUpdate run) >>= k_tgt)
 
@@ -578,7 +579,7 @@ Section SIM.
     { guclo sim_itree_indC_spec. econs 8; eauto. gbase. eauto. }
     { guclo sim_itree_indC_spec. econs 9; eauto. des. esplits; eauto. gbase. eauto. }
     { guclo sim_itree_indC_spec. econs 10; eauto. gbase. eauto. }
-    { guclo sim_itree_indC_spec. econs 11; eauto. gbase. eauto. }
+    { guclo sim_itree_indC_spec. econs 11; eauto.  gbase. eauto. }
   Qed.
 
   Lemma sim_itreeC_spec r g
@@ -629,136 +630,149 @@ Section SIM.
     { exploit SRC0; auto. exploit TGT0; auto. i. clarify. econs; eauto. }
   Qed.
 
-  (* If src/tgt itree is different from each other, how does the relation change? *)
-  (* In which case "st_src =/= st_tgt" holds? (Isn't it always same?)*)
-  Definition sim_fsem: relation (option mname * Any.t -> itree (Es st) Any.t) :=
+  Definition respectful' := fun (A B C D: Type) (R: A -> B -> Prop) (R': C -> D -> Prop) (f: A -> C) (g: B -> D) => forall x y, R x y -> R' (f x) (g y).
+
+  Definition sim_fsem {st_src st_tgt} (wf: world -> st_src * st_tgt -> Prop): (Any.t -> itree (Es st_src) Any.t) -> (Any.t -> itree (Es st_tgt) Any.t) -> Prop :=
+    (respectful' eq (fun it_src it_tgt => forall w mrs_src mrs_tgt
+    (SIMMRS: wf w (mrs_src, mrs_tgt)), 
+    sim_itree false false w wf (mrs_src, it_src) (mrs_tgt, it_tgt)
+    ))%signature.
+
+
+  (* Definition sim_fsem: relation (option mname * Any.t -> itree (Es st) Any.t) :=
     (eq ==> (fun it_src it_tgt => forall w mrs_src mrs_tgt (SIMMRS: wf w (mrs_src, mrs_tgt)),
                  sim_itree false false w (mrs_src, it_src)
                            (mrs_tgt, it_tgt)))%signature
-  .
+  . *)
 
-  Definition sim_fnsem: relation (string * (option mname * Any.t -> itree (Es st) Any.t)) := RelProd eq sim_fsem.
+  Definition sim_fnsem {st_src st_tgt} (wf: world -> st_src * st_tgt -> Prop): (gname -> option (Any.t -> itree (Es st_src) Any.t)) -> (gname -> option (Any.t -> itree (Es st_tgt) Any.t)) -> Prop :=
+    fun f g => forall s, match (f s), (g s) with
+                        | Some x, Some y => sim_fsem wf x y
+                        | None, None => True
+                        | _, _ => False
+                        end
+    .
+
+  (* Definition sim_fnsem: relation (string * (option mname * Any.t -> itree (Es st) Any.t)) := RelProd eq sim_fsem. *)
 
 
-  Variant lflagC (r: forall (R_src R_tgt: Type) (RR: st_local -> st_local -> R_src -> R_tgt -> Prop), bool -> bool -> world -> st_local * itree (Es st) R_src -> st_local * itree (Es st) R_tgt -> Prop)
-          {R_src R_tgt} (RR: st_local -> st_local -> R_src -> R_tgt -> Prop)
-    : bool -> bool -> world -> st_local * itree (Es st) R_src -> st_local * itree (Es st) R_tgt -> Prop :=
+  Variant lflagC (r: forall (st_src st_tgt R_src R_tgt: Type) (wf: world -> st_src * st_tgt -> Prop)
+    (RR: st_src -> st_tgt -> R_src -> R_tgt -> Prop), bool -> bool -> world -> st_src * itree (Es st_src) R_src -> st_tgt * itree (Es st_tgt) R_tgt -> Prop)
+          {st_src st_tgt R_src R_tgt} (wf: world -> st_src * st_tgt -> Prop) (RR: st_src -> st_tgt -> R_src -> R_tgt -> Prop)
+    : bool -> bool -> world -> st_src * itree (Es st_src) R_src -> st_tgt * itree (Es st_tgt) R_tgt -> Prop :=
   | lflagC_intro
       f_src0 f_src1 f_tgt0 f_tgt1 w st_src st_tgt
-      (SIM: r _ _ RR f_src0 f_tgt0 w st_src st_tgt)
+      (SIM: r _ _ _ _ wf RR f_src0 f_tgt0 w st_src st_tgt)
       (SRC: f_src0 = true -> f_src1 = true)
       (TGT: f_tgt0 = true -> f_tgt1 = true)
     :
-      lflagC r RR f_src1 f_tgt1 w st_src st_tgt
+      lflagC r wf RR f_src1 f_tgt1 w st_src st_tgt
   .
 
   Lemma lflagC_mon
         r1 r2
-        (LE: r1 <8= r2)
+        (LE: r1 <11= r2)
     :
-      @lflagC r1 <8= @lflagC r2
+      @lflagC r1 <11= @lflagC r2
   .
   Proof. ii. destruct PR; econs; et. Qed.
 
   Hint Resolve lflagC_mon: paco.
 
-  Lemma lflagC_spec: lflagC <9= gupaco8 (_sim_itree) (cpn8 _sim_itree).
+  Lemma lflagC_spec: lflagC <12= gupaco11 (_sim_itree) (cpn11 _sim_itree).
   Proof.
-    eapply wrespect8_uclo; eauto with paco.
+    eapply wrespect11_uclo; eauto with paco.
     econs; eauto with paco. i. inv PR.
     eapply GF in SIM.
-    revert x3 x4 SRC TGT. induction SIM using _sim_itree_ind2; i; clarify.
+    revert x6 x7 SRC TGT. induction SIM using _sim_itree_ind2; i; clarify.
     { econs 1; eauto. }
     { econs 2; eauto. i. exploit K; eauto. i. des.
-      esplits; eauto. eapply rclo8_base. eauto. }
-    { econs 3; eauto. i. eapply rclo8_base. eauto. }
+      esplits; eauto. eapply rclo11_base. eauto. }
+    { econs 3; eauto. i. eapply rclo11_base. eauto. }
     { econs 4; eauto. }
-    { econs 5; eauto. des. esplits; eauto. }
-    { econs 6; eauto. i. exploit K; eauto. i. des. esplits; eauto. }
-    { econs 7; eauto. }
-    { econs 8; eauto. }
-    { econs 9; eauto. }
-    { econs 10; eauto. i. exploit K; eauto. i. des. esplits; eauto. }
-    { econs 11; eauto. des. esplits; eauto. }
-    { econs 12; eauto. }
-    { econs 13; eauto. }
-    { exploit SRC0; auto. exploit TGT0; auto. i. clarify. econs 14; eauto.
-      eapply rclo8_base; auto. }
+    { econs 5; eauto. }
+    { econs 6; eauto.  des. esplits; eauto. }
+    { econs 7; eauto. i. exploit K; eauto. i. des. esplits; eauto. }
+    { econs 8; eauto. i. exploit K; eauto. i. des. esplits; eauto. }
+    { econs 9; eauto. des. esplits; eauto. }
+    { econs 10; eauto. }
+    { econs 11; eauto. }
+    { exploit SRC0; auto. exploit TGT0; auto. i. clarify. econs 12; eauto.
+      eapply rclo11_base; auto. }
   Qed.
 
-  Lemma sim_itree_flag_down R0 R1 RR r g w st_src st_tgt f_src f_tgt
-        (SIM: gpaco8 _sim_itree (cpn8 _sim_itree) r g R0 R1 RR false false w st_src st_tgt)
+  Lemma sim_itree_flag_down {st_src st_tgt} R0 R1 (wf: world -> st_src * st_tgt -> Prop) RR r g w st_src0 st_tgt0 f_src f_tgt
+        (SIM: gpaco11 _sim_itree (cpn11 _sim_itree) r g _ _ R0 R1 wf RR false false w st_src0 st_tgt0)
     :
-      gpaco8 _sim_itree (cpn8 _sim_itree) r g R0 R1 RR f_src f_tgt w st_src st_tgt.
+      gpaco11 _sim_itree (cpn11 _sim_itree) r g _ _ R0 R1 wf RR f_src f_tgt w st_src0 st_tgt0.
   Proof.
     guclo lflagC_spec. econs; eauto.
   Qed.
 
-  Lemma sim_itree_bot_flag_up R0 R1 RR w st_src st_tgt f_src f_tgt
-        (SIM: paco8 _sim_itree bot8 R0 R1 RR true true w st_src st_tgt)
+  Lemma sim_itree_bot_flag_up {st_src st_tgt} R0 R1 (wf: world -> st_src * st_tgt -> Prop) RR w st_src0 st_tgt0 f_src f_tgt
+        (SIM: paco11 _sim_itree bot11 _ _ R0 R1 wf RR true true w st_src0 st_tgt0)
     :
-      paco8 _sim_itree bot8 R0 R1 RR f_src f_tgt w st_src st_tgt.
+      paco11 _sim_itree bot11 _ _ R0 R1 wf RR f_src f_tgt w st_src0 st_tgt0.
   Proof.
     ginit. remember true in SIM at 1. remember true in SIM at 1.
-    clear Heqb Heqb0. revert w st_src st_tgt f_src f_tgt b b0 SIM.
-    gcofix CIH. i. revert f_src f_tgt.
+    clear Heqb Heqb0. revert w st_src0 st_tgt0 f_src f_tgt b b0 SIM.
+    gcofix CIH. 
+    i. revert f_src f_tgt.
 
     (* TODO: why induction using sim_itree_ind doesn't work? *)
-    pattern b, b0, w, st_src, st_tgt.
+    pattern b, b0, w, st_src0, st_tgt0.
     match goal with
-    | |- ?P b b0 w st_src st_tgt => set P
+    | |- ?P b b0 w st_src0 st_tgt0 => set P
     end.
-    revert b b0 w st_src st_tgt SIM.
-    eapply (@sim_itree_ind R0 R1 RR P); subst P; ss; i; clarify.
+    revert b b0 w st_src0 st_tgt0 SIM.
+    eapply (@sim_itree_ind _ _ R0 R1 wf RR P); subst P; ss; i; clarify.
     { guclo sim_itree_indC_spec. econs 1; eauto. }
     { gstep. econs 2; eauto. i. gbase. eapply CIH; eauto. }
     { gstep. econs 3; eauto. i. gbase. eapply CIH; eauto. }
     { guclo sim_itree_indC_spec. econs 4; eauto. }
-    { guclo sim_itree_indC_spec. econs 5; eauto. des. esplits; eauto. }
-    { guclo sim_itree_indC_spec. econs 6; eauto. i. hexploit K; eauto. i. des. esplits; eauto. }
-    { guclo sim_itree_indC_spec. econs 7; eauto. }
-    { guclo sim_itree_indC_spec. econs 8; eauto. }
-    { guclo sim_itree_indC_spec. econs 9; eauto. }
-    { guclo sim_itree_indC_spec. econs 10; eauto. i. hexploit K; eauto. i. des. esplits; eauto. }
-    { guclo sim_itree_indC_spec. econs 11; eauto. des. esplits; eauto. }
-    { guclo sim_itree_indC_spec. econs 12; eauto. }
-    { guclo sim_itree_indC_spec. econs 13; eauto. }
+    { guclo sim_itree_indC_spec. econs 5; eauto. } 
+    { guclo sim_itree_indC_spec. econs 6; eauto. des. esplits; eauto. }
+    { guclo sim_itree_indC_spec. econs 7; eauto. i. hexploit K; eauto. i. des. esplits; eauto. }
+    { guclo sim_itree_indC_spec. econs 8; eauto. i. hexploit K; eauto. i. des. esplits; eauto. }
+    { guclo sim_itree_indC_spec. econs 9; eauto. des. esplits; eauto. }
+    { guclo sim_itree_indC_spec. econs 10; eauto. } 
+    { guclo sim_itree_indC_spec. econs 11; eauto. } 
     { eapply sim_itree_flag_down. gfinal. right.
-      eapply paco8_mon; eauto. ss.
+      eapply paco11_mon; eauto. ss.
     }
   Qed.
 
-  Variant lbindR (r s: forall S_src S_tgt (SS: st_local -> st_local -> S_src -> S_tgt -> Prop), bool -> bool -> world -> st_local * itree (Es st) S_src -> st_local * itree (Es st) S_tgt -> Prop):
-    forall S_src S_tgt (SS: st_local -> st_local -> S_src -> S_tgt -> Prop), bool -> bool -> world -> st_local * itree (Es st) S_src -> st_local * itree (Es st) S_tgt -> Prop :=
+  Variant lbindR (r s: forall st_src st_tgt S_src S_tgt (wf: world -> st_src * st_tgt -> Prop) (SS: st_src -> st_tgt -> S_src -> S_tgt -> Prop), bool -> bool -> world -> st_src * itree (Es st_src) S_src -> st_tgt * itree (Es st_tgt) S_tgt -> Prop):
+    forall st_src st_tgt S_src S_tgt (wf: world -> st_src * st_tgt -> Prop) (SS: st_src -> st_tgt -> S_src -> S_tgt -> Prop), bool -> bool -> world -> st_src * itree (Es st_src) S_src -> st_tgt * itree (Es st_tgt) S_tgt -> Prop :=
   | lbindR_intro
       f_src f_tgt w0 w1
-
-      R_src R_tgt RR
-      (st_src0 st_tgt0: st_local)
-      (i_src: itree (Es st) R_src) (i_tgt: itree (Es st) R_tgt)
-      (SIM: r _ _ RR f_src f_tgt w0 (st_src0, i_src) (st_tgt0, i_tgt))
+      st_src st_tgt
+      R_src R_tgt wf RR
+      (st_src0: st_src )(st_tgt0: st_tgt)
+      (i_src: itree (Es st_src) R_src) (i_tgt: itree (Es st_tgt) R_tgt)
+      (SIM: r _ _ _ _ wf RR f_src f_tgt w0 (st_src0, i_src) (st_tgt0, i_tgt))
 
       S_src S_tgt SS
-      (st_src0, k_src: ktree (Es st) R_src S_src) (st_tgt0, k_tgt: ktree (Es st) R_tgt S_tgt)
-      (SIMK: forall st_src1 st_tgt1 vret_src vret_tgt (SIM: RR st_src1 st_tgt1 vret_src vret_tgt), s _ _ SS false false w1 (st_src1, k_src vret_src) (st_tgt1, k_tgt vret_tgt))
+      (k_src: ktree (Es st_src) R_src S_src) (k_tgt: ktree (Es st_tgt) R_tgt S_tgt)
+      (SIMK: forall st_src1 st_tgt1 vret_src vret_tgt (SIM: RR st_src1 st_tgt1 vret_src vret_tgt), s _ _ _ _ wf SS false false w1 (st_src1, k_src vret_src) (st_tgt1, k_tgt vret_tgt))
     :
-      lbindR r s SS f_src f_tgt w1 (st_src0, ITree.bind i_src k_src) (st_tgt0, ITree.bind i_tgt k_tgt)
+      lbindR r s wf SS f_src f_tgt w1 (st_src0, ITree.bind i_src k_src) (st_tgt0, ITree.bind i_tgt k_tgt)
   .
 
   Hint Constructors lbindR: core.
 
-  Lemma lbindR_mon
+  Lemma lbindR_mon 
         r1 r2 s1 s2
-        (LEr: r1 <8= r2) (LEs: s1 <8= s2)
+        (LEr: r1 <11= r2) (LEs: s1 <11= s2)
     :
-      lbindR r1 s1 <8= lbindR r2 s2
+      lbindR r1 s1 <11= lbindR r2 s2
   .
   Proof. ii. destruct PR; econs; et. Qed.
 
   Definition lbindC r := lbindR r r.
   Hint Unfold lbindC: core.
 
-  Lemma lbindC_wrespectful: wrespectful8 (_sim_itree) lbindC.
+  Lemma lbindC_wrespectful: wrespectful11 (_sim_itree) lbindC.
   Proof.
     econs.
     { ii. eapply lbindR_mon; eauto. }
@@ -769,38 +783,36 @@ Section SIM.
     induction SIM using _sim_itree_ind2; i; clarify.
     + rewrite ! bind_ret_l. exploit SIMK; eauto. i.
       eapply sim_itree_flag_mon.
-      { eapply sim_itree_mon; eauto. i. eapply rclo8_base. auto. }
+      { eapply sim_itree_mon; eauto. i. eapply rclo11_base. auto. }
       { ss. }
       { ss. }
     + rewrite ! bind_bind. econs; eauto. i.
-      eapply rclo8_clo_base. econs; eauto.
+      eapply rclo11_clo_base. econs; eauto.
     + rewrite ! bind_bind. econs; eauto. i.
-      eapply rclo8_clo_base. econs; eauto.
+      eapply rclo11_clo_base. econs; eauto.
+    + rewrite ! bind_tau. econs; eauto.
     + rewrite ! bind_tau. econs; eauto.
     + rewrite ! bind_bind. econs; eauto. des. esplits; eauto.
     + rewrite ! bind_bind. econs; eauto. i. exploit K; eauto. i. des. esplits; eauto.
-    + rewrite ! bind_bind. econs; eauto.
-    + rewrite ! bind_bind. econs; eauto.
-    + rewrite ! bind_tau. econs; eauto.
     + rewrite ! bind_bind. econs; eauto. i. exploit K; eauto. i. des. esplits; eauto.
     + rewrite ! bind_bind. econs; eauto. des. esplits; eauto.
-    + rewrite ! bind_bind. econs; eauto.
-    + rewrite ! bind_bind. econs; eauto.
-    + econs; eauto. eapply rclo8_clo_base. econs; eauto.
+    + rewrite ! bind_bind. econs; eauto. 
+    + rewrite ! bind_bind. econs; eauto. 
+    + econs; eauto. eapply rclo11_clo_base. econs; eauto.
   Qed.
 
-  Lemma lbindC_spec: lbindC <9= gupaco8 (_sim_itree) (cpn8 (_sim_itree)).
+  Lemma lbindC_spec: lbindC <12= gupaco11 (_sim_itree) (cpn11 (_sim_itree)).
   Proof.
-    intros. eapply wrespect8_uclo; eauto with paco. eapply lbindC_wrespectful.
+    intros. eapply wrespect11_uclo; eauto with paco. eapply lbindC_wrespectful.
   Qed.
 
 End SIM.
 Hint Resolve sim_itree_mon: paco.
-Hint Resolve cpn8_wcompat: paco.
+Hint Resolve cpn11_wcompat: paco.
 
 Lemma self_sim_itree:
-  forall st itr,
-    sim_itree (fun _ '(src, tgt) => src = tgt) top2 false false tt (st, itr) (st, itr).
+  forall st st0 itr,
+    @sim_itree unit top2 st st false false tt (fun _ '(src, tgt) => src = tgt) (st0, itr) (st0, itr).
 Proof.
   ginit. gcofix CIH. i. ides itr.
   { gstep. eapply sim_itree_ret; ss. }
@@ -814,22 +826,18 @@ Proof.
     eapply sim_itree_flag_down. gbase. auto.
   }
   destruct s.
-  { rewrite <- ! bind_trigger. resub. dependent destruction p.
-    { guclo sim_itree_indC_spec. econs.
-      guclo sim_itree_indC_spec. econs.
-      eapply sim_itree_progress_flag. gbase. auto.
-    }
+  { rewrite <- ! bind_trigger. resub. dependent destruction s.
     { guclo sim_itree_indC_spec. econs.
       guclo sim_itree_indC_spec. econs.
       eapply sim_itree_progress_flag. gbase. auto.
     }
   }
   { rewrite <- ! bind_trigger. resub. dependent destruction e.
-    { guclo sim_itree_indC_spec. econs 10. i.
+    { guclo sim_itree_indC_spec. econs 7. i.
       guclo sim_itree_indC_spec. econs. eexists.
       eapply sim_itree_progress_flag. gbase. eauto.
     }
-    { guclo sim_itree_indC_spec. econs 6. i.
+    { guclo sim_itree_indC_spec. econs 8. i.
       guclo sim_itree_indC_spec. econs. eexists.
       eapply sim_itree_progress_flag. gbase. eauto.
     }
@@ -838,7 +846,6 @@ Proof.
     }
   }
 Qed.
-
 
 
 (*** desiderata: (1) state-aware simulation relation !!!! ***)
@@ -852,15 +859,17 @@ Section SIMMODSEM.
 
   Variable (ms_src ms_tgt: ModSem.t).
 
-  Let W: Type := (Any.t) * (Any.t).
+  Let W: Type := (ms_src.(ModSem.state)) * (ms_tgt.(ModSem.state)).
+
   Inductive sim: Prop := mk {
     world: Type;
     wf: world -> W -> Prop;
     le: world -> world -> Prop;
     le_PreOrder: PreOrder le;
-    sim_fnsems: Forall2 (sim_fnsem wf le) ms_src.(ModSem.fnsems) ms_tgt.(ModSem.fnsems);
-    sim_mn: ms_src.(ModSem.mn) = ms_tgt.(ModSem.mn);
-    sim_initial: exists w_init, wf w_init (ms_src.(ModSem.initial_st), ms_tgt.(ModSem.initial_st));
+    sim_fnsems: (sim_fnsem le wf) (ms_src.(ModSem.fnsems)) (ms_tgt.(ModSem.fnsems));
+    (* sim_fnsems: Forall2 (sim_fnsem wf le) ms_src.(ModSem.fnsems) ms_tgt.(ModSem.fnsems); *)
+    (* sim_mn: ms_src.(ModSem.mn) = ms_tgt.(ModSem.mn); *)
+    sim_initial: exists w_init, wf w_init (ms_src.(ModSem.init_st), ms_tgt.(ModSem.init_st));
   }.
 
 End SIMMODSEM.
@@ -871,14 +880,16 @@ Proof.
   econs; et.
   - instantiate (1:=fun (_ _: unit) => True). ss.
   - instantiate (1:=(fun (_: unit) '(src, tgt) => src = tgt)). (* fun p => fst p = snd p *)
-    generalize (ModSem.fnsems ms).
+    admit.
+    (* generalize (ModSem.fnsems ms). 
     induction l; ii; ss.
     econs; eauto. econs; ss. ii; clarify.
-    destruct w. exploit self_sim_itree; et.
+    destruct w. exploit self_sim_itree; et. *)
   - ss.
-Unshelve.
+Admitted.
+  (* Unshelve.
 all: try (exact 0).
-Qed.
+Qed. *)
 
 End ModSemPair.
 
@@ -913,23 +924,23 @@ Section SIMMOD.
 
   Lemma ModL_add_fnsems md0 md1 sk
     :
-      (ModSemL.fnsems (ModL.get_modsem (ModL.add md0 md1) sk)) =
-      (ModSemL.fnsems (ModL.get_modsem md0 sk)) ++ (ModSemL.fnsems (ModL.get_modsem md1 sk)).
+      (ModSem.fnsems (Mod.get_modsem (Mod.add md0 md1) sk)) =
+      ModSem.add_fnsems (Mod.get_modsem md0 sk) (Mod.get_modsem md1 sk).
   Proof.
     ss.
   Qed.
 
-  Lemma ModL_add_sk md0 md1
+  Lemma Mod_add_sk md0 md1
     :
-      ModL.sk (ModL.add md0 md1) = ModL.sk md0 ++ ModL.sk md1.
+      Mod.sk (Mod.add md0 md1) = Mod.sk md0 ++ Mod.sk md1.
   Proof.
     ss.
   Qed.
 
-  Lemma Mod_list_incl_sk (mds: list Mod.t) md
+  (* Lemma Mod_list_incl_sk (mds: list Mod.t) md
         (IN: In md mds)
     :
-      Sk.incl (Mod.sk md) (ModL.sk (Mod.add_list mds)).
+      Sk.incl (Mod.sk md) (Mod.sk (Mod.add_list mds)).
   Proof.
     rewrite Mod.add_list_sk. revert IN. induction mds; ss.
     i. des; clarify.
@@ -939,13 +950,13 @@ Section SIMMOD.
 
   Lemma Mod_add_list_get_modsem (mds: list Mod.t) sk
     :
-      ModL.get_modsem (Mod.add_list mds) sk
+      Mod.get_modsem (Mod.add_list mds) sk
       =
-      fold_right ModSemL.add {| ModSemL.fnsems := []; ModSemL.initial_mrs := [] |}
-                 (List.map (fun (md: Mod.t) => ModL.get_modsem md sk) mds).
+      fold_right ModSem.add {| ModSem.fnsems := []; ModSem.initial_mrs := [] |}
+                 (List.map (fun (md: Mod.t) => Mod.get_modsem md sk) mds).
   Proof.
     induction mds; ss. f_equal. rewrite <- IHmds. ss.
-  Qed.
+  Qed. *)
 
 End SIMMOD.
 
@@ -968,81 +979,87 @@ Import TAC.
 
 Section ADEQUACY.
   Section SEMPAIR.
-    Variable ms_src: ModSemL.t.
-    Variable ms_tgt: ModSemL.t.
+    Variable ms_src: ModSem.t.
+    Variable ms_tgt: ModSem.t.
 
-    Variable mn: mname.
+    (* Variable mn: mname. *)
     Variable world: Type.
-    Variable wf: world -> Any.t * Any.t -> Prop.
+    Let W: Type := (ms_src.(ModSem.state)) * (ms_tgt.(ModSem.state)). 
+    (* Variable wf: world -> W -> Prop.  *)
+    (* Variable wf: world -> Any.t * Any.t -> Prop. *)
     Variable le: world -> world -> Prop.
 
     Hypothesis le_PreOrder: PreOrder le.
 
-    Hypothesis fnsems_find_iff:
-      forall fn,
-        (<<NONE: alist_find fn ms_src.(ModSemL.fnsems) = None>>) \/
-        (exists mn' (f: _ -> itree _ _),
-            (<<MN: mn <> mn'>>) /\
-            (<<SRC: alist_find fn ms_src.(ModSemL.fnsems) = Some (transl_all mn' (T:=Any.t) ∘ f)>>) /\
-            (<<TGT: alist_find fn ms_tgt.(ModSemL.fnsems) = Some (transl_all mn' (T:=Any.t) ∘ f)>>)) \/
+    Hypothesis fnsems_find_iff :
+      forall fn (wf: world -> W -> Prop),
+        (<<NONE: ms_src.(ModSem.fnsems) fn = None>>) \/
+        (* (exists (f: _ -> itree _ _),
+            (* (<<MN: mn <> mn'>>) /\ *)
+            (<<SRC: ms_src.(ModSem.fnsems) fn = Some (f)>>) /\
+            (<<TGT: ms_tgt.(ModSem.fnsems) fn = Some (f)>>)) \/ *)
         (exists (f_src f_tgt: _ -> itree _ _),
-            (<<SRC: alist_find fn ms_src.(ModSemL.fnsems) = Some (transl_all mn (T:=Any.t) ∘ f_src)>>) /\
-            (<<TGT: alist_find fn ms_tgt.(ModSemL.fnsems) = Some (transl_all mn (T:=Any.t) ∘ f_tgt)>>) /\
-            (<<SIM: sim_fsem wf le f_src f_tgt>>)).
+            (<<SRC: ms_src.(ModSem.fnsems) fn = Some (f_src)>>) /\
+            (<<TGT: ms_tgt.(ModSem.fnsems) fn = Some (f_tgt)>>) /\
+            (<<SIM: sim_fsem le wf f_src f_tgt>>)).
 
 
     Variant g_lift_rel
-            (w0: world) (st_src st_tgt: p_state): Prop :=
+            (w0: world) (wf: world -> W -> Prop ) st_src0 st_tgt0: Prop :=
     | g_lift_rel_intro
         w1
         (LE: le w0 w1)
-        (MN: wf w1 (st_src mn, st_tgt mn))
-        (NMN: forall mn' (NIN: mn <> mn'), st_src mn' = st_tgt mn')
+        (MN: wf w1 (st_src0, st_tgt0))
+        (* (NMN: forall mn' (NIN: mn <> mn'), st_src mn' = st_tgt mn') *)
     .
 
     Variant my_r0:
       forall R0 R1 (RR: R0 -> R1 -> Prop), bool -> bool -> (itree eventE R0) -> (itree eventE R1) -> Prop :=
     | my_r0_intro
-        w0
-        (itr_src itr_tgt: itree (Es st) Any.t)
-        st_src st_tgt o_src o_tgt
-        (SIM: sim_itree wf le o_src o_tgt w0 (st_src mn, itr_src) (st_tgt mn, itr_tgt))
-        (STATE: forall mn' (MN: mn <> mn'), st_src mn' = st_tgt mn')
+        w0 (wf: world -> W -> Prop )
+        (st_src: Type := ms_src.(ModSem.state)) (st_tgt: Type := ms_tgt.(ModSem.state))
+        (itr_src: itree (Es st_src) Any.t)(itr_tgt: itree (Es st_tgt) Any.t)
+        st_src0 st_tgt0 o_src o_tgt
+        (SIM: sim_itree le o_src o_tgt w0 wf (st_src0, itr_src) (st_tgt0, itr_tgt))
+        (* (STATE: forall mn' (MN: mn <> mn'), st_src mn' = st_tgt mn') *)
       :
         my_r0 (fun '(st_src, ret_src) '(st_tgt, ret_tgt) =>
-                 g_lift_rel w0 st_src st_tgt /\ ret_src = ret_tgt)
+                  g_lift_rel w0 wf st_src st_tgt /\ ret_src = ret_tgt)
               o_src o_tgt
-              (EventsL.interp_Es (ModSemL.prog ms_src) (transl_all mn itr_src) st_src)
-              (EventsL.interp_Es (ModSemL.prog ms_tgt) (transl_all mn itr_tgt) st_tgt)
+              (interp_Es (ModSem.prog ms_src) (itr_src) st_src0)
+              (interp_Es (ModSem.prog ms_tgt) (itr_tgt) st_tgt0)
     .
 
-    Variant my_r1:
+    (* Variant my_r1:
       forall R0 R1 (RR: R0 -> R1 -> Prop), bool -> bool -> (itree eventE R0) -> (itree eventE R1) -> Prop :=
     | my_r1_intro
-        mn' w0 st_src st_tgt
-        (MN: mn <> mn')
-        (SIM: g_lift_rel w0 st_src st_tgt)
-        (itr: itree (Es st) Any.t)
+        w0
+        (st_src: Type := ms_src.(ModSem.state)) (st_tgt: Type := ms_tgt.(ModSem.state))
+        st_src0 st_tgt0
+        (wf: world -> W -> Prop)
+        (* (MN: mn <> mn') *)
+        (SIM: g_lift_rel w0 wf st_src0 st_tgt0)
+        (itr_src: itree (Es st_src) Any.t)
+        (itr_tgt: itree (Es st_tgt) Any.t)
       :
-        my_r1 (fun '(st_src, ret_src) '(st_tgt, ret_tgt) =>
-                 g_lift_rel w0 st_src st_tgt /\ ret_src = ret_tgt)
+        my_r1 (fun '(st_src0, ret_src) '(st_tgt0, ret_tgt) =>
+                 g_lift_rel w0 wf st_src0 st_tgt0 /\ ret_src = ret_tgt)
               false false
-              (EventsL.interp_Es (ModSemL.prog ms_src) (transl_all mn' itr) st_src)
-              (EventsL.interp_Es (ModSemL.prog ms_tgt) (transl_all mn' itr) st_tgt)
-    .
+              (interp_Es (ModSem.prog ms_src) (itr_src) st_src0)
+              (interp_Es (ModSem.prog ms_tgt) (itr_tgt) st_tgt0)
+    . *)
 
-    Let my_r := my_r0 \7/ my_r1.
-    Let sim_lift: my_r <7= simg.
+    (* Let my_r := my_r0 \7/ my_r1. *)
+    Let sim_lift: my_r0 <7= simg.
     Proof.
       ginit.
       { i. eapply cpn7_wcompat; eauto with paco. }
       gcofix CIH. i. destruct PR.
-      { destruct H.
         unfold sim_itree in SIM.
-        remember (st_src mn, itr_src).
-        remember (st_tgt mn, itr_tgt).
+        remember (st_src0, itr_src).
+        remember (st_tgt0, itr_tgt).
         remember w0 in SIM at 2.
-        revert st_src itr_src st_tgt itr_tgt Heqp Heqp0 Heqw STATE.
+        revert st_src0 itr_src st_tgt0 itr_tgt Heqp Heqp0 Heqw.
 
         (* TODO: why induction using sim_itree_ind doesn't work? *)
         pattern o_src, o_tgt, w, p, p0.
@@ -1050,52 +1067,47 @@ Section ADEQUACY.
         | |- ?P o_src o_tgt w p p0 => set P
         end.
         revert o_src o_tgt w p p0 SIM.
-        eapply (@sim_itree_ind world wf le Any.t Any.t (lift_rel wf le w0 (@eq Any.t)) P); subst P; ss; i; clarify.
+        eapply (@sim_itree_ind world le _ _ Any.t Any.t wf (lift_rel le w0 wf (@eq Any.t)) P); subst P; ss; i; clarify.
 
         - rr in RET. des. step. splits; auto. econs; et.
         - hexploit (fnsems_find_iff fn). i. des.
-          { steps. rewrite NONE. unfold unwrapU, triggerUB. step. ss. }
-          { steps. rewrite SRC. rewrite TGT. unfold unwrapU. ired_both.
+          { step. rewrite interp_Es_bind.  steps. rewrite NONE. unfold unwrapU, triggerUB. (* step.: coq bug?????? *) rewrite interp_Es_bind. step.  ss. }
+          (* { ired_both. step. rewrite interp_Es_bind. ired_both. steps. rewrite SRC. rewrite TGT. unfold unwrapU. ired_both.
             apply simg_progress_flag.
             guclo bindC_spec. econs.
             { gbase. eapply CIH. right. econs; ss. econs; et. refl. }
-            { i. ss. des. destruct vret_src, vret_tgt. des; clarify. inv SIM.
-              hexploit K; et. i. des. pclearbot.
-              steps. gbase. eapply CIH. left. econs; et.
+            { i. ss. des. destruct vret_src, vret_tgt. des; clarify. inv SIM0.
+              hexploit K; et. i. des. pclearbot. ired_both. ired_both. guclo simg_safe_spec. econs. et; i.
+
+              step. gbase. eapply CIH. left. econs; et.
             }
-          }
-          { hexploit (SIM (Some mn, varg) (Some mn, varg)); et. i. des.
-            steps. rewrite SRC. rewrite TGT. unfold unwrapU. ired_both.
+          } *)
+          { hexploit (SIM (varg) (varg)); et. i. des. ired_both. 
+            steps. rewrite interp_Es_bind. rewrite SRC. rewrite TGT. unfold unwrapU. ired_both.
             apply simg_progress_flag.
             guclo bindC_spec. econs.
-            { gbase. eapply CIH. left. econs; ss. et. }
+            { gbase. eapply CIH. econs; ss. rewrite bind_ret_l. rewrite bind_ret_r. et. }
             { i. ss. destruct vret_src, vret_tgt. des; clarify. inv SIM0.
-              hexploit K; et. i. des. pclearbot.
-              steps. gbase. eapply CIH. left. econs; et.
+              hexploit K; et. i. des. pclearbot. ired_both.
+              steps. gbase. eapply CIH. econs; et.
             }
           }
         - step. i. subst. apply simg_progress_flag.
           hexploit (K x_tgt). i. des. pclearbot.
-          steps. gbase. eapply CIH. left. econs; et.
-        - ired_both. steps.
-        - des. force. exists x. steps. eapply IH; eauto.
-        - steps. i. hexploit K. i. des. steps. eapply IH; eauto.
-        - steps. eapply IH; eauto.
-          { unfold update. des_ifs. }
-          { i. unfold update. des_ifs. et. }
-        - steps. eapply IH; eauto.
+          steps. gbase. eapply CIH. econs; et.
         - steps.
+        - steps. 
+        - des. force. exists x. steps. eapply IH; eauto. 
+        - steps. i. hexploit K. i. des. steps. eapply IH; eauto.
         - steps. i. hexploit K. i. des. steps. eapply IH; eauto.
         - des. force. exists x. steps. eapply IH; eauto.
-        - steps. eapply IH; eauto.
-          { unfold update. des_ifs. }
-          { i. unfold update. des_ifs. et. }
-        - steps. eapply IH; eauto.
-        - eapply simg_progress_flag. gbase. eapply CIH.
-          left. econs; eauto.
-      }
-      { destruct H. ides itr.
-        { steps. }
+        - steps. destruct run. steps. eapply IH; eauto.
+        - steps. destruct run. steps. eapply IH; eauto.
+        - eapply simg_progress_flag. gbase. eapply CIH. econs; eauto.
+    Qed.
+    (* my_r1 ??? *)
+      (* { destruct H. ides itr.
+        { steps. split; et. }
         { steps. eapply simg_progress_flag. gbase. eapply CIH. right. econs; et. }
         rewrite <- ! bind_trigger. destruct e.
         { resub. destruct c. hexploit (fnsems_find_iff fn). i. des.
@@ -1147,24 +1159,24 @@ Section ADEQUACY.
             gbase. eapply CIH; et. right. econs; et. }
         }
       }
-    Qed.
+    Qed. *)
 
     Context `{CONF: EMSConfig}.
 
-    Hypothesis INIT:
-      exists w, g_lift_rel w (ModSemL.initial_p_state ms_src) (ModSemL.initial_p_state ms_tgt).
+    (* Hypothesis INIT:
+      exists w, g_lift_rel w (ModSem.initial_p_state ms_src) (ModSem.initial_p_state ms_tgt). *)
 
     Lemma adequacy_local_aux (P Q: Prop)
           (WF: Q -> P)
       :
-        (Beh.of_program (ModSemL.compile ms_tgt (Some P)))
+        (Beh.of_program (ModSem.compile ms_tgt (Some P)))
         <1=
-        (Beh.of_program (ModSemL.compile ms_src (Some Q))).
-    Proof.
-      eapply adequacy_global_itree; ss.
+        (Beh.of_program (ModSem.compile ms_src (Some Q))).
+    Proof. Admitted.
+      (* eapply adequacy_global_itree; ss.
       hexploit INIT. i. des. ginit.
       { eapply cpn7_wcompat; eauto with paco. }
-      unfold ModSemL.initial_itr, assume.
+      unfold ModSem.initial_itr, assume.
       hexploit (fnsems_find_iff "main"). i. des.
       { steps. unshelve esplits; et. unfold ITree.map, unwrapU, triggerUB. steps.
         rewrite NONE. steps. ss. }
@@ -1183,7 +1195,7 @@ Section ADEQUACY.
         { i. destruct vret_src, vret_tgt. des; clarify. steps. }
       }
       Unshelve. all: try exact 0.
-    Qed.
+    Qed. *)
   End SEMPAIR.
 
   Theorem adequacy_local_strong md_src md_tgt
@@ -1191,16 +1203,16 @@ Section ADEQUACY.
     :
       <<CR: (refines_strong md_tgt md_src)>>
   .
-  Proof.
-    ii. unfold ModL.compile, ModL.enclose in *.
-    destruct (classic (ModL.wf (ModL.add (Mod.add_list ctx) md_src))).
-    2:{ eapply ModSemL.compile_not_wf. ss. }
-    pose (sk_tgt := (ModL.sk (ModL.add (Mod.add_list ctx) md_tgt))).
-    pose (sk_src := (ModL.sk (ModL.add (Mod.add_list ctx) md_src))).
+  Proof. Admitted.
+    (* ii. unfold Mod.compile, Mod.enclose in *.
+    destruct (classic (Mod.wf (Mod.add (Mod.add_list ctx) md_src))).
+    2:{ eapply ModSem.compile_not_wf. ss. }
+    pose (sk_tgt := (Mod.sk (Mod.add (Mod.add_list ctx) md_tgt))).
+    pose (sk_src := (Mod.sk (Mod.add (Mod.add_list ctx) md_src))).
     assert (SKEQ: sk_tgt = sk_src).
     { unfold sk_src, sk_tgt. ss. f_equal.
       inv SIM. auto. }
-    rr in H. unfold ModL.enclose in *. fold sk_src in H. des. inv WF.
+    rr in H. unfold Mod.enclose in *. fold sk_src in H. des. inv WF.
     rename SK into SKWF.
     rename wf_fnsems into FNWF.
     rename wf_initial_mrs into MNWF.
@@ -1210,8 +1222,8 @@ Section ADEQUACY.
       unfold Sk.wf in *. ss. eapply Permutation.Permutation_NoDup; [|et].
       eapply Permutation.Permutation_map. eapply Sk.SkSort.sort_permutation. }
     i. inv H. des.
-    assert (WFTGT: ModL.wf (ModL.add (Mod.add_list ctx) md_tgt)).
-    { rr. unfold ModL.enclose. fold sk_src sk_tgt.
+    assert (WFTGT: Mod.wf (Mod.add (Mod.add_list ctx) md_tgt)).
+    { rr. unfold Mod.enclose. fold sk_src sk_tgt.
       rewrite SKEQ in *. split; auto. econs.
       { clear MNWF.
         match goal with
@@ -1260,7 +1272,7 @@ Section ADEQUACY.
     }
     { exists w_init. econs.
       { refl. }
-      { unfold ModSemL.initial_p_state.
+      { unfold ModSem.initial_p_state.
         erewrite ! alist_find_some_iff; et.
         { clear FNWF.
           match goal with
@@ -1272,11 +1284,11 @@ Section ADEQUACY.
         { ss. eapply in_or_app. right. ss. left. fold sk_tgt. f_equal. auto. }
         { ss. eapply in_or_app. right. ss. left. fold sk_src. rewrite SKEQ. auto. }
       }
-      { ii. ss. fold sk_src sk_tgt. rewrite SKEQ. unfold ModSemL.initial_p_state.
+      { ii. ss. fold sk_src sk_tgt. rewrite SKEQ. unfold ModSem.initial_p_state.
         ss. rewrite ! alist_find_app_o. des_ifs_safe.
         rewrite <- SKEQ. ss. rewrite ! eq_rel_dec_correct. des_ifs. }
     }
-  Qed.
+  Qed. *)
 
   Context {CONF: EMSConfig}.
 
@@ -1296,17 +1308,17 @@ Section ADEQUACY.
     :
       <<CR: refines_strong (Mod.add_list mds_tgt) (Mod.add_list mds_src)>>
   .
-  Proof.
-    r. induction FORALL; ss.
+  Proof. Admitted.
+    (* r. induction FORALL; ss.
     { ii. auto. }
-    rewrite ! Mod.add_list_cons.
+    (* rewrite ! Mod.add_list_cons. *)
     etrans.
     { rewrite <- Mod.add_list_single. eapply refines_strong_proper_r.
       rewrite ! Mod.add_list_single. eapply adequacy_local_strong; et. }
     replace (Mod.lift x) with (Mod.add_list [x]); cycle 1.
-    { cbn. rewrite ModL.add_empty_r. refl. }
+    { cbn. rewrite Mod.add_empty_r. refl. }
     eapply refines_strong_proper_l; et.
-  Qed.
+  Qed. *)
 
   Theorem adequacy_local2 md_src md_tgt
           (SIM: ModPair.sim md_src md_tgt)
