ems/SimGlobal.v
@@ -691,8 +691,8 @@ Let ms_src: ModSem.t := md_src.(Mod.enclose).
 Let ms_tgt: ModSem.t := md_tgt.(Mod.enclose).
 
 Section ADEQUACY.
-Hypothesis (SIM: simg eq false false (@ModSem.initial_itr ms_src CONFS ) (@ModSem.initial_itr ms_tgt CONFT )).
-(* Hypothesis (SIM: simg eq false false (@ModSem.initial_itr ms_src CONFS (Some (Mod.wf md_src))) (@ModSem.initial_itr ms_tgt CONFT (Some (Mod.wf md_tgt)))). *)
+(* Hypothesis (SIM: simg eq false false (@ModSem.initial_itr ms_src CONFS ) (@ModSem.initial_itr ms_tgt CONFT )). *)
+Hypothesis (SIM: simg eq false false (@ModSem.initial_itr ms_src CONFS (Some (Mod.wf md_src))) (@ModSem.initial_itr ms_tgt CONFT (Some (Mod.wf md_tgt)))).
 
 
 Theorem adequacy_global: Beh.of_program (@Mod.compile _ CONFT md_tgt) <1= Beh.of_program (@Mod.compile _ CONFS md_src).
