spc/Hoareproof2.v
@@ -36,41 +36,64 @@ Section CANCEL.
 
   Context `{Σ: GRA.t}.
 
-  Variable mds: list SMod.t.
+  (* Variable mds: list SMod.t. *)
+  Variable md: SMod.t.
 
-  Let sk: Sk.t := Sk.sort (fold_right Sk.add Sk.unit (List.map SMod.sk mds)).
+  (* Let sk: Sk.t := Sk.sort (fold_right Sk.add Sk.unit (List.map SMod.sk mds)). *)
+  Let sk: Sk.t := Sk.add Sk.unit (SMod.sk md).
   (* Let skenv: SkEnv.t := Sk.load_skenv sk. *)
-  Let mss: list SModSem.t := (List.map ((flip SMod.get_modsem) sk) mds).
-  Let sbtb: list (gname * fspecbody) := (List.flat_map (SModSem.fnsems) mss).
-  Let _stb: list (gname * fspec) := List.map (fun '(fn, fs) => (fn, fs.(fsb_fspec))) sbtb.
+  (* Let mss: list SModSem.t := (List.map ((flip SMod.get_modsem) sk) mds). *)
+  Let ms: SModSem.t := (SMod.get_modsem md) sk.
+  (* Let sbtb: list (gname * fspecbody) := (List.flat_map (SModSem.fnsems) mss). *)
+  Let sbtb := SModSem.fnsems ms.
+  (* Let _stb: list (gname * fspec) := List.map (fun '(fn, fs) => (fn, fs.(fsb_fspec))) sbtb. *)
+  Let _stb := fun fn => match (sbtb fn) with
+                      | None => None 
+                      | Some fsb => Some (fsb_fspec fsb)
+                      end
+  .
 
   Variable stb: gname -> option fspec.
+  (* Hypothesis STBCOMPLETE:
+    forall fn fsp (FIND: alist_find fn _stb = Some fsp), stb fn = Some fsp. *)
   Hypothesis STBCOMPLETE:
-    forall fn fsp (FIND: alist_find fn _stb = Some fsp), stb fn = Some fsp.
-  Hypothesis STBSOUND:
+    forall fn fsp (FIND: _stb fn = Some fsp), stb fn = Some fsp.
+
+  (* Hypothesis STBSOUND:
     forall fn (FIND: alist_find fn _stb = None),
+      (<<NONE: stb fn = None>>) \/ (exists fsp, <<FIND: stb fn = Some fsp>> /\ <<TRIVIAL: forall x, fsp.(measure) x = ord_top>>). *)
+
+  Hypothesis STBSOUND:
+    forall fn (FIND: _stb fn = None),
       (<<NONE: stb fn = None>>) \/ (exists fsp, <<FIND: stb fn = Some fsp>> /\ <<TRIVIAL: forall x, fsp.(measure) x = ord_top>>).
 
 
-  Let mds_src: list Mod.t := List.map (SMod.to_src) mds.
-  Let mds_mid2: list Mod.t := List.map (SMod.to_mid2 stb) mds.
+  (* Let mds_src: list Mod.t := List.map (SMod.to_src) mds.
+  Let mds_mid2: list Mod.t := List.map (SMod.to_mid2 stb) mds. *)
 
-
+  Let md_src: Mod.t := SMod.to_src md.
+  Let md_mid2: Mod.t := SMod.to_mid2 stb md.
 
   Let W: Type := p_state.
 
-  Opaque EventsL.interp_Es.
+  Opaque interp_Es.
 
-  Let ms_src: ModSemL.t := ModL.enclose (Mod.add_list mds_src).
-  Let ms_mid2: ModSemL.t := ModL.enclose (Mod.add_list mds_mid2).
+  (* Let ms_src: ModSemL.t := ModL.enclose (Mod.add_list mds_src).
+  Let ms_mid2: ModSemL.t := ModL.enclose (Mod.add_list mds_mid2). *)
 
-  Let p_src := ModSemL.prog ms_src.
-  Let p_mid2 := ModSemL.prog ms_mid2.
+  Let ms_src: ModSem.t := Mod.enclose md_src.
+  Let ms_mid2: ModSem.t := Mod.enclose md_mid2.
+
+  (* Let p_src := ModSemL.prog ms_src.
+  Let p_mid2 := ModSemL.prog ms_mid2. *)
+
+  Let p_src := ModSem.prog ms_src.
+  Let p_mid2 := ModSem.prog ms_mid2.
 
   Require Import IRed.
 
 
-  Lemma my_lemma__APC o (w: unit) st
+  (* Lemma my_lemma__APC o (w: unit) st
     :
       paco8 (_sim_itree (fun (_: unit) '(st_src, st_tgt) => st_src = st_tgt) top2) bot8 unit unit
             (fun st_src st_tgt _ _ => st_src = st_tgt)
@@ -85,29 +108,69 @@ Section CANCEL.
     { my_steps. }
     my_steps. deflag.
     eapply IH; auto.
+  Qed. *)
+
+  Lemma my_lemma__APC o (w: unit) st (st0: st)
+    :
+      paco11 (_sim_itree top2) bot11 _ _ unit unit (fun (_: unit) '(st_src0, st_tgt0) => st_src0 = st_tgt0)
+            (fun st_src0 st_tgt0 _ _ => st_src0 = st_tgt0)
+            false false w
+            (st0, Ret tt)
+            (st0, interp_hCallE_mid2 (_APC _ o)).
+  Proof.
+    ginit. revert w st0.
+    induction (Ord.lt_well_founded o); i. clear H. rename x into o. rename H0 into IH.
+    rewrite unfold_APC. my_steps.
+    destruct x.
+    { my_steps. }
+    my_steps. deflag. eapply IH; auto. 
+    (* rewrite interp_mid2_bind. rewrite interp_mid2_triggere. rewrite bind_bind. 
+    apply sim_itreeC_spec. eapply sim_itreeC_choose_tgt. i. rewrite bind_tau.
+    apply sim_itreeC_spec. eapply sim_itreeC_tau_tgt. rewrite bind_ret_l.
+    rewrite interp_mid2_bind. rewrite interp_mid2_guarantee. rewrite bind_bind.
+    unfold guarantee. rewrite bind_bind. 
+    apply sim_itreeC_spec. eapply sim_itreeC_choose_tgt. rewrite bind_ret_l. rewrite bind_tau. i.
+    apply sim_itreeC_spec. eapply sim_itreeC_tau_tgt. rewrite bind_ret_l.
+    rewrite interp_mid2_bind. rewrite interp_mid2_triggere. rewrite bind_bind.
+    apply sim_itreeC_spec. eapply sim_itreeC_choose_tgt. i. rewrite bind_tau. 
+    apply sim_itreeC_spec. eapply sim_itreeC_tau_tgt. rewrite bind_ret_l. 
+    destruct x1. rewrite interp_mid2_bind. ired_r.
+    apply sim_itreeC_spec. eapply sim_itreeC_tau_tgt. 
+    apply sim_itreeC_spec. eapply sim_itreeC_choose_tgt. i. rewrite bind_tau.
+    apply sim_itreeC_spec. eapply sim_itreeC_tau_tgt. rewrite bind_ret_l.
+    eapply IH; auto. *)
   Qed.
 
   Lemma idK_spec2: forall E A B (a: A) (itr: itree E B), itr = Ret a >>= fun _ => itr. Proof. { i. ired. ss. } Qed.
 
   Context {CONF: EMSConfig}.
   Theorem adequacy_type_m2s:
-    Beh.of_program (ModL.compile (Mod.add_list mds_mid2)) <1=
-    Beh.of_program (ModL.compile (Mod.add_list mds_src)).
+    Beh.of_program (Mod.compile md_mid2) <1=
+    Beh.of_program (Mod.compile md_src).
   Proof.
     eapply ModSem.refines_close.
-    eapply (@adequacy_local_list_strong mds_src mds_mid2).
-    unfold mds_src, mds_mid2.
-    eapply Forall2_apply_Forall2.
-    { refl. }
-    i. subst. econs; ss. i. econs; ss.
+    eapply (@adequacy_local_strong md_src md_mid2).
+    (* eapply (@adequacy_local_list_strong mds_src mds_mid2). *)
+    unfold md_src, md_mid2.
+    
+    (* eapply Forall2_apply_Forall2. *)
+    (* { refl. } *)
+    econs; ss. econs; ss.
     { instantiate (1:=fun (_ _: unit) => True). ss. }
-    { instantiate (1:=fun _ '(st_src, st_tgt) => st_src = st_tgt).
-      eapply Forall2_apply_Forall2.
-      { refl. }
-      i. subst. destruct b0. econs; ss. ii. subst.
+    { instantiate (1:=fun _ '(st_src, st_tgt) => st_src = st_tgt). ii. des_ifs.
+    
+  
+
+
+      (* eapply Forall2_apply_Forall2. *)
+      (* { refl. } *)
+      (* destruct b0.  *)
+      (* econs; ss. *)
+       ii. subst.
       unfold fun_to_src, fun_to_mid2, body_to_src, body_to_mid2. ss.
       generalize (fsb_body f y).
       revert mrs_tgt w. ginit. gcofix CIH. i. ides i.
+      (* { rewrite interp_hEs_tgt_ret, interp_mid2_ret, interp_src_ret. steps. } *)
       { steps. }
       { steps. deflag. gbase. eapply CIH. }
       rewrite <- bind_trigger.
@@ -117,7 +180,7 @@ Section CANCEL.
         force_r. i. ired_both.
         steps. deflag. rewrite (idK_spec2 tt (interp_hEs_src (k ()))).
         guclo lbindC_spec. econs.
-        { deflag. gfinal. right. eapply paco8_mon.
+        { deflag. gfinal. right. eapply paco11_mon.
           { eapply my_lemma__APC. }
           { i. ss. }
         }
@@ -130,13 +193,13 @@ Section CANCEL.
         deflag. gbase. et.
       }
       destruct s0.
-      { resub. destruct p.
+      { resub. destruct s0.
         { ired_both. force_r. force_l. steps.
           deflag. gbase. et.
         }
-        { ired_both. force_r. force_l. steps.
+        (* { ired_both. force_r. force_l. steps.
           deflag. gbase. et.
-        }
+        } *)
       }
       { resub. destruct e.
         { ired_both. force_r. i. force_l. exists x. steps.
